some progress towards restoring regressions; StreamPlain, AEAD_GCM and StreamAE are still broken

src/tls/StreamAE.fst
@@ -4,9 +4,6 @@ module StreamAE
 // plaintexts; concretely, we use AES_GCM but any other AEAD algorithm
 // would do.
 
-// This implementations *assumes* "Stateful AE" security, then calls CoreCrypto
-// Alternatively, we should go down to AEAD with noAD. 
-
 open FStar.Heap
 open FStar.HyperHeap
 open FStar.Seq
@@ -22,30 +19,17 @@ open TLSConstants
 open TLSInfo
 open StreamPlain
 
+
 let gen parent i = 
   let kv = CoreCrypto.random (CoreCrypto.aeadKeySize (alg i)) in
   let iv = CoreCrypto.random (iv_length i) in
   let writer_r = new_region parent in
   if authId i then 
-    begin 
-      let log : ideal_log writer_r i = alloc_mref_seq writer_r Seq.createEmpty in
-      let h = ST.get() in
-      assert(0 <= max_seqn); 
-      assert(0 <= Seq.length (m_sel #writer_r #(s:seq (entry i){True}) h log));
-      let ectr: ideal_seqn writer_r i log = new_seqn writer_r 0 max_seqn log in
-
-      //16-09-13 can we avoid the coercion below?
-      let log : maybe_log writer_r i = to_maybe_log log in 
-      let w = State #i #Writer #writer_r #writer_r kv iv log ectr in
-
-      //16-09-13 these are now needed to prove the (authID ==> ...) postcondition
-      let h1 = ST.get() in 
-      assert(m_contains #writer_r #(s:seq (entry i){True}) (ilog w.log) h1);
-      assert(m_sel h1 (ilog w.log) == createEmpty);
-      w
-    end
+    let log : ideal_log writer_r i = alloc_mref_seq writer_r Seq.createEmpty in
+    let ectr: ideal_ctr writer_r i log = new_seqn writer_r 0 log in
+    State #i #Writer #writer_r #writer_r kv iv log ectr
   else 
-    let ectr: concrete_seqn writer_r i = m_alloc writer_r 0 in
+    let ectr: concrete_ctr writer_r i = m_alloc writer_r 0 in
     State #i #Writer #writer_r #writer_r kv iv () ectr 
 
 
@@ -54,17 +38,14 @@ let genReader parent #i w =
   if authId i
   then
     let log : ideal_log w.region i = w.log in
-    let h = ST.get() in
-    assert(0 <= max_seqn); 
-    assert(0 <= Seq.length (m_sel #w.region #(s:seq (entry i){True}) h log));
-    let dctr: ideal_seqn reader_r i log = new_seqn reader_r 0 max_seqn log in
+    let dctr: ideal_ctr reader_r i log = new_seqn reader_r 0 log in
     State #i #Reader #reader_r #(w.region) w.key w.iv w.log dctr
-  else let dctr : concrete_seqn reader_r i = m_alloc reader_r 0 in
+  else let dctr : concrete_ctr reader_r i = m_alloc reader_r 0 in
     State #i #Reader #reader_r #(w.region) w.key w.iv () dctr
 
 let coerce parent i kv iv =
   let writer_r = new_region parent in
-  let ectr: concrete_seqn writer_r i = m_alloc writer_r 0 in
+  let ectr: concrete_ctr writer_r i = m_alloc writer_r 0 in
   State #i #Writer #writer_r #writer_r kv iv () ectr 
 
 let leak #i #role s = State.key s, State.iv s
@@ -79,9 +60,9 @@ let leak #i #role s = State.key s, State.iv s
 //
 // The XORing is a fixed, ad hoc, random permutation; not sure what is gained;
 // we can reason about sequence-number collisions before applying it.
-let aeIV i (seqn:seqnum) (staticIV:iv i) : lbytes (iv_length i) =
+let aeIV i (seqn:counter) (staticIV:iv i) : lbytes (iv_length i) =
   lemma_repr_bytes_values seqn;
-  max_seqn_value ();
+  max_ctr_value ();
   let extended = bytes_of_int (iv_length i) seqn in
   xor (iv_length i) extended staticIV
 
@@ -93,9 +74,8 @@ let noAD = empty_bytes
    safeId i is fixed to false and after removal of the cryptographic ghost log,
    i.e. all idealization is turned off *)
 let encrypt #i e l p =
-  let ctr = ctr e.seqn in 
+  let ctr = ctr e.counter in 
   m_recall ctr;
-  assume(safeId i <==> authId i); //TODO elsewhere
   let text = if safeId i then createBytes l 0z else repr i l p in
   let n = m_read ctr in
   let iv = aeIV i n e.iv in
@@ -104,56 +84,45 @@ let encrypt #i e l p =
     begin
     let ilog = ilog e.log in
     m_recall ilog;
-    let ictr: ideal_seqn e.region i ilog = e.seqn in
-    testify_seqn ictr; //now we know that j <= Seq.length log
-    let h = ST.get() in 
-    m_recall ilog;
+    let ictr: ideal_ctr e.region i ilog = e.counter in
+    testify_seqn ictr;
+    write_at_end ilog (Entry l c p); //need to extend the log first, before incrementing the counter for monotonicity; do this only if ideal
     m_recall ictr;
-    assert(m_sel h ictr <= Seq.length (m_sel h ilog)); 
-    write_at_end ilog (Entry l c p); //need to extend the log first, before incrementing the seqn for monotonicity; do this only if ideal
-    let h = ST.get() in
-    assert (m_sel h ictr < Seq.length (m_sel h ilog)); 
-    m_recall ictr;
-    increment_seqn (fun _ -> True) ictr;
+    increment_seqn ictr;
     m_recall ictr
     end
   else
     m_write ctr (n + 1);
   c
 
-#set-options "--z3timeout 10000"
-// decryption, idealized as a lookup at index d.seq# in the log for safe instances
+
+// decryption, idealized as a lookup of (c,ad) in the log for safe instances
 let decrypt #i d l c =
-  let ctr = ctr d.seqn in 
+  let ctr = ctr d.counter in 
   m_recall ctr;
   let j = m_read ctr in
   if authId i 
   then 
     let ilog = ilog d.log in
     let log  = m_read ilog in
-    let ictr: ideal_seqn d.region i ilog = d.seqn in
+    let ictr: ideal_ctr d.region i ilog = d.counter in
     let _ = testify_seqn ictr in //now we know that j <= Seq.length log
     if j < Seq.length log && matches l c (Seq.index log j) then
       begin
-      increment_seqn (fun _ -> True) ictr;
+      increment_seqn ictr;
       m_recall ctr;
       Some (Entry.p (Seq.index log j))
       end
     else None
   else //concrete
      let iv = aeIV i j d.iv in
-     let o = CoreCrypto.aead_decrypt (alg i) d.key iv noAD c in 
-     match o with
+     match CoreCrypto.aead_decrypt (alg i) d.key iv noAD c with
      | None -> None
      | Some pr ->
        begin
-         let a = alg i in 
-         //16-09-13  can't prove a precondition below, why?
-         assert(c = CoreCrypto.aead_encryptT a d.key iv noAD pr);
-         assert(length c = length pr + CoreCrypto.aeadTagSize a);
-         match mk_plain i l pr with
-         | Some p -> (m_write ctr (j + 1); Some p)
-         | None   -> None
+       match mk_plain i l pr with
+       | Some p -> (m_write ctr (j + 1); Some p)
+       | None   -> None
        end
 
 
