src/tls/StreamAE.fsti
@@ -1,8 +1,7 @@
 module StreamAE
 
 // Authenticated encryption for a stream of variable-length plaintexts.
-// Supports all TLS 1.3 record protection mechanisms (but aims at generality)
-// No support for additional authenticated data.
+// Concretely, we use AES_GCM but any other algorithm would do.
 
 open FStar.Heap
 open FStar.HyperHeap
@@ -21,112 +20,78 @@ open StreamPlain
 
 module HH = FStar.HyperHeap
 
-// The index is treated abstractly, with
-// - a restriction to TLS 1.3
-// - `alg` for controlling algorithmic agility (consider making it private)
-
 type id = i:id { is_ID13 i }
+
 let alg (i:id) : CoreCrypto.aead_cipher = AEAD._0 (aeAlg_of_id i)
+
+let ltag i : nat = CoreCrypto.aeadTagSize (alg i)
+
+let cipherLen i (l:plainLen) : nat = l + ltag i
+
+type cipher i (l:plainLen) = lbytes (cipherLen i l)
+
+// will require proving before decryption
+let lenCipher i (c:bytes { ltag i <= length c }) : nat = length c - ltag i
+
+type entry (i:id) =
+  | Entry: l:plainLen -> c:cipher i l -> p:plain i l -> entry i
 
 private inline let min (a:int) (b:int) = if a < b then a else b
 private inline let max (a:int) (b:int) = if a < b then b else a
-
-
-(*** Key materials ***)
 
 // The length of the per-record nonce (iv_length) is set to max(8 bytes, N_MIN)
 // for the AEAD algorithm (see [RFC5116] Section 4)
 let iv_length i = max 8 (CoreCrypto.aeadRealIVSize (alg i))
 
-// concrete representations
+// key materials 
 type key (i:id) = lbytes (CoreCrypto.aeadKeySize (alg i)) 
 type iv  (i:id) = lbytes (iv_length i)
 
-
-(*** Plaintexts and ciphertexts ***)
-
-// Plaintexts are defined in StreamPlain, represented as bounded bytestrings.
-// Ciphertexts are longer by exactly (tagLen i) bytes.
-
-let tagLen i : nat = CoreCrypto.aeadTagSize (alg i)
-let cipherLen i (l:plainLen) : nat = l + tagLen i
-type cipher i (l:plainLen) = lbytes (cipherLen i l)
-
-// Presumed plaintext length when decrypting c
-let lenCipher i (c:bytes { tagLen i <= length c }) : nat = length c - tagLen i
-
-//16-09-10 causing a lexing error, why? 
-//(* ** Ideal State ***) 
-
-// ideal StreamAE maintains a table from sequence numbers to entries
-// (we'll need a separate ideal flag to support dynamic compromise)
-
-
-type entry (i:id) =
-  | Entry: l:plainLen -> c:cipher i l -> p:plain i l -> entry i
-
-
 let ideal_log (r:rid) (i:id) = log_t r (entry i)
 
-let maybe_log (r:rid) (i:id) : Tot Type0 =
+let log_ref (r:rid) (i:id) : Tot Type0 =
   if authId i then ideal_log r i else unit
 
-// applied to force generalization (?)
-let to_maybe_log (#r:rid) (#i:id) (l:ideal_log r i{authId i}) : maybe_log r i = l
+let ilog (#r:rid) (#i:id) (l:log_ref r i{authId i}) : Tot (ideal_log r i) =
+  l
 
-// applied to force the condition within maybe_log
-let ilog (#r:rid) (#i:id) (l:maybe_log r i{authId i}) : Tot (ideal_log r i) = l
+irreducible let max_ctr: nat = pow2 64 - 1
 
-// 'ctr' here refers to the encryption sequence number---not the internal block counter.
+assume val max_ctr_value: unit -> Lemma (max_ctr = 18446744073709551615)
 
-irreducible let max_seqn: nat = pow2 64 - 1
-assume val max_seqn_value: unit -> Lemma (max_seqn = 18446744073709551615)
-// how to avoid this?
+type counter = c:nat{c <= max_ctr} 
 
-type seqnum = c:nat{c <= max_seqn} 
+let ideal_ctr (#l:rid) (r:rid) (i:id) (log:ideal_log l i) : Tot Type0 =
+  FStar.Monotonic.Seq.seqn r log max_ctr
+  // An increasing counter, at most min(length log, 2^64-1)
+  
+let concrete_ctr (r:rid) (i:id) : Tot Type0 = 
+  m_rref r counter increases
 
-// a ref to an increasing sequence number,
-// when authId i, the sequence number is at most min(length log, max_seqn)
-
-let concrete_seqn (r:rid) (i:id) : Tot Type0 = m_rref r seqnum increases
-
-let ideal_seqn (#rl:rid) (r:rid) (i:id) (log:ideal_log rl i) : Tot Type0 =
-  FStar.Monotonic.Seq.seqn r log max_seqn
-    
-let maybe_seqn (#rl:rid) (r:rid) (i:id) (log:maybe_log rl i) : Tot Type0 = 
+let ctr_ref (#l:rid) (r:rid) (i:id) (log:log_ref l i) : Tot Type0 = 
   if authId i   
-  then ideal_seqn r i (log <: ideal_log rl i)
-  else m_rref r seqnum increases
+  then ideal_ctr r i (log <: ideal_log l i)
+  else m_rref r counter increases
 
-let ctr (#rl:rid) (#r:rid) (#i:id) (#log:maybe_log rl i) (c:maybe_seqn r i log)
+let ctr (#l:rid) (#r:rid) (#i:id) (#log:log_ref l i) (c:ctr_ref r i log)
   : Tot (m_rref r (if authId i 
-		   then seqn_val #rl #(entry i) #(fun (s:seq (entry i)) -> True) r (ilog log) max_seqn 
-		   else seqnum) 
+		   then seqn_val #l #(entry i) r log max_ctr 
+		   else counter) 
 		increases) =
   c
 
-(*
-// error message: on log:
-exp (FStar.Monotonic.Seq.i_seq rl (StreamAE.entry i) (fun s -> Prims.l_True))
-got (StreamAE.maybe_log l i)
-  = if authId i then ideal_log rl i else unit
-  = log_t rl (entry i) 
-  = i_seq rl a (fun (s:seq a) -> True) (fun s -> True)
-*)
-
-// local state for encryption and decryption.
-// kept concrete for log and seqn, but key and iv should be private.
+// kept concrete for log and counter, but the key and iv should be private.
 noeq type state (i:id) (rw:rw) = 
   | State: #region: rgn
          -> #log_region: rgn{if rw = Writer then region = log_region else HyperHeap.disjoint region log_region}
          -> key: key i
          -> iv: iv i
-         -> log: maybe_log log_region i     // ghost, subject to cryptographic assumption
-         -> seqn: maybe_seqn region i log // types are sufficient to anti-alias log and seqn
+         -> log: log_ref log_region i // ghost, subject to cryptographic assumption
+         -> counter: ctr_ref region i log // types are sufficient to anti-alias log and counter
          -> state i rw
 
 // Some invariants:
-// - the writer seqn is the length of the log; the reader seqn is lower or equal
+// - the writer counter is the length of the log; the reader counter is lower or equal
 // - gen is called at most once for each (i:id), generating distinct refs for each (i:id)
 // - the log is monotonic
 
@@ -143,8 +108,8 @@ let genPost (#i:id) parent h0 (w:writer i) h1 =
   (authId i ==>
       (m_contains (ilog w.log) h1 /\
        m_sel h1 (ilog w.log) == createEmpty)) /\
-  m_contains (ctr w.seqn) h1 /\
-  m_sel h1 (ctr w.seqn) === 0
+  m_contains (ctr w.counter) h1 /\
+  m_sel h1 (ctr w.counter) === 0
 //16-04-30 how to share the whole ST ... instead of genPost?
 
 // Generate a fresh instance with index i in a fresh sub-region of r0
@@ -162,11 +127,11 @@ val genReader: parent:rid -> #i:id -> w:writer i -> ST (reader i)
                HH.parent r.region = parent /\
 	       color r.region = color parent /\
                fresh_region r.region h0 h1 /\
-               op_Equality #(maybe_log w.region i) w.log r.log /\
-	       m_contains (ctr r.seqn) h1 /\
-	       m_sel h1 (ctr r.seqn) === 0))
+               op_Equality #(log_ref w.region i) w.log r.log /\
+	       m_contains (ctr r.counter) h1 /\
+	       m_sel h1 (ctr r.counter) === 0))
 // encryption (on concrete bytes), returns (cipher @| tag)
-// Keeps seqn and nonce implicit; requires the seqn not to overflow
+// Keeps seqn and nonce implicit; requires the counter not to overflow
 // encryption of plaintexts; safe instances are idealized
 
 
@@ -176,16 +141,18 @@ val coerce: parent:rid -> i:id{~(authId i)} -> kv:key i -> iv:iv i -> ST (writer
   (requires (fun h0 -> True))
   (ensures  (genPost parent))
 
+
 val leak: #i:id{~(authId i)} -> #role:rw -> state i role -> ST (key i * iv i)
   (requires (fun h0 -> True))
   (ensures  (fun h0 r h1 -> modifies Set.empty h0 h1 ))
 
+
 val encrypt: #i:id -> e:writer i -> l:plainLen -> p:plain i l -> ST (cipher i l)
-  (requires (fun h0 -> m_sel h0 (ctr e.seqn) < max_seqn))
-  (ensures  (fun h0 c h1 ->
+    (requires (fun h0 -> m_sel h0 (ctr e.counter) < max_ctr))
+    (ensures  (fun h0 c h1 ->
                  modifies_one e.region h0 h1 /\
-                 m_contains (ctr e.seqn) h1 /\
-                 m_sel h1 (ctr e.seqn) === m_sel h0 (ctr e.seqn) + 1 /\
+                 m_contains (ctr e.counter) h1 /\
+                 m_sel h1 (ctr e.counter) === m_sel h0 (ctr e.counter) + 1 /\
 	         (authId i ==>
 		   (let log = ilog e.log in
 		    let ent = Entry l c p in
@@ -199,12 +166,12 @@ let matches (#i:id) (l:plainLen) (c:cipher i l) (e:entry i) : Tot bool =
   let Entry l' c' _ = e in
   l = l' && c = c'
 
-// decryption, idealized as a lookup at index d.seq# in the log for safe instances
+// decryption, idealized as a lookup of (c,ad) in the log for safe instances
 val decrypt: #i:id -> d:reader i -> l:plainLen -> c:cipher i l
   -> ST (option (plain i (min l (max_TLSPlaintext_fragment_length + 1))))
-  (requires (fun h0 -> m_sel h0 (ctr d.seqn) < max_seqn))
+  (requires (fun h0 -> m_sel h0 (ctr d.counter) < max_ctr))
   (ensures  (fun h0 res h1 ->
-      let j = m_sel h0 (ctr d.seqn) in
+      let j = m_sel h0 (ctr d.counter) in
       (authId i ==>
 	(let log = m_sel h0 (ilog d.log) in
 	 if j < Seq.length log && matches l c (Seq.index log j)
@@ -213,5 +180,5 @@ val decrypt: #i:id -> d:reader i -> l:plainLen -> c:cipher i l
     /\ (match res with
        | None -> modifies Set.empty h0 h1
        | _  ->   modifies_one d.region h0 h1
-              /\ modifies_rref d.region !{as_ref (as_rref (ctr d.seqn))} h0 h1
-	      /\ m_sel h1 (ctr d.seqn) === j + 1)))
+              /\ modifies_rref d.region !{as_ref (as_rref (ctr d.counter))} h0 h1
+	      /\ m_sel h1 (ctr d.counter) === j + 1)))
